Modified storage and proof structures, advanced proofs resolutions

Distributed/paper_implementation.lean
@@ -1,11 +1,63 @@
 -- Structures useful to define our data structure
 namespace Model
 
-def Set (n: Nat) (T: Type) := (Fin n) -> T
+def Map (n: Nat) (T: Type) := (Fin n) -> T
 
-def updateSet [BEq T] (f: (Fin n) -> T) (i: Fin n) (t: T): (Fin n) -> T:=
+def updateMap [BEq T] (f: Map n T) (i: Fin n) (t: T): (Fin n) -> T:=
     λ x => if i == x then t else f x
 
+def Set (n: Nat) := Map n Bool
+
+def emptySet : Set n:= λ _ => false
+
+def insertElem (s: Set n) (i: Fin n) := updateMap s i true
+
+def contains (s: Set n) (i: Fin n): Bool := s i
+
+
+def count_ (s: Set n) (i: Nat) (h: NeZero n): Nat :=
+  match i with
+  | 0 => 0
+  | a + 1 =>
+    if s (Fin.ofNat n a) then 1 + count_ s a h else  count_ s a h
+   
+
+def count (s: Set n): Nat :=
+  if h : (n ≠ 0) then
+     have : NeZero n := ⟨h⟩ 
+     count_ s n this
+  else
+        0
+
+
+theorem fullSetImpN (s: Set n):
+count s = n
+-> ∀ i, s i = true := by
+   sorry
+   
+   
+   
+   
+
+theorem setAcceptNotIncr (s: Set n) (h: n ≠ 0) :
+∀ i, s i = true
+-> ∀ i, count (insertElem s i) = n := by
+   intros i sIsTrue i'
+   simp [count]; split; grind
+   unfold count_ insertElem updateMap
+   sorry
+   
+theorem fullSetCannotIncrease (s: Set n):
+count s = n
+-> ∀ i, count (insertElem s i) = n := by 
+   induction n
+   intro sZero i; unfold count at *; grind
+   rename_i n IH; intro countN i;
+   have cc : (n +1 ≠ 0) := by {grind}
+   apply (setAcceptNotIncr s cc)
+   apply (fullSetImpN s countN); apply i
+
+   
 
 inductive Preference where 
 | Yes : Preference
@@ -26,8 +78,8 @@ deriving BEq, DecidableEq
 structure Coordinator (n: Nat) where
 numParticipants : Nat := n
 decision: Option Decision
-yesVotes: Array Bool
-noVotes: Array Bool
+yesVotes: Set n
+noVotes: Set n
 
 structure Participant (n: Nat) where
 hostid: (Fin n)
@@ -38,9 +90,10 @@ deriving BEq, DecidableEq
 structure Network (n : Nat) where
 network: List (Message n)
 
-structure System where
-n: Nat
+structure System (n: Nat) where
 coordinator: Coordinator n
-participants: Set n (Participant n)
+participants: Map n (Participant n)
 network: Network n
+
+
 
