Distributed/paper_proofs.lean
@@ -6,16 +6,16 @@ open Model
 
 -- Init properties: Check that the program has a valid init state
 def coordinatorInits (c: Coordinator n) : Prop :=
-    c.decision = none ∧ c.yesVotes = Array.replicate n false ∧ c.noVotes = Array.replicate n false
+    c.decision = none ∧ c.yesVotes = emptySet ∧ c.noVotes = emptySet
 
-def participantInits (p: Participant n): Prop :=
-    p.decision = none
+def participantInits (p: Participant n) (idx: Fin n): Prop :=
+    p.decision = none ∧ (p.hostid = idx)
 
 def networkInits (n: Network n): Prop :=
     n.network = []
 
-def systemInits (s: System) : Prop :=
-    networkInits s.network ∧ coordinatorInits s.coordinator ∧ ∀ i, participantInits (s.participants i)
+def systemInits (s: System n) : Prop :=
+    networkInits s.network ∧ coordinatorInits s.coordinator ∧ ∀ i, participantInits (s.participants i) i
 
 -- Steps: list all possible steps
 
@@ -25,16 +25,16 @@ snd = Message.Vote p1.preference p1.hostid ∧ p2 = p1
 def CoordinatorReceivesPreference(c1: Coordinator n) (c2: Coordinator n) (rcv: Message n): Prop:= 
     ∃ (pref: Model.Preference) (id: Fin n), rcv = Message.Vote pref id
     ∧ if pref = Preference.Yes then
-      c2 = {c1 with yesVotes := c1.yesVotes.insertIdx! id.toNat true}
+      c2 = {c1 with yesVotes := insertElem c1.yesVotes id}
     else
-      c2 = {c1 with noVotes := c1.noVotes.insertIdx! id.toNat true}    
+      c2 = {c1 with noVotes := insertElem c1.noVotes id}    
 
 
 def CoordinatorMakesDecisionStep (c1: Coordinator n) (c2: Coordinator n) : Prop:=
 c1.decision = none ∧
-if c1.yesVotes.count true == n then
+if count c1.yesVotes = n  then
    c2 = {c1 with decision := some Decision.Commit}
-else if c1.noVotes.count true  >= 1 then
+else if count c1.noVotes >= 1 then
    c2 = {c1 with decision := some Decision.Abort}
 else
    c2 = c1
@@ -46,24 +46,34 @@ def ParticipantReceiveDecisionStep (p1: Participant n) (p2: Participant n) (m: M
 ∃ a, m = Message.Decide a ∧ p1.decision = none ∧ p2 = {p1 with decision := some a}
 
 
-inductive step : System -> System -> Prop where
-| partSendPref: ∀ (s: System) i p2 snd, ParticipantSendsPreference (s.participants i) p2 snd -> step s {s with participants := updateSet s.participants i p2, network := {s.network with network := snd :: s.network.network}}
-| coordRecvPref: ∀ (s: System) c2 rcv , CoordinatorReceivesPreference s.coordinator c2 rcv -> step s {s with coordinator := c2, network := {s.network with network := s.network.network.erase rcv}}
-| coordMksDec: ∀ s c2, CoordinatorMakesDecisionStep s.coordinator c2 -> step s {s with coordinator := c2}
-| coordSndDecStep: ∀ (s: System) snd, CoordinatorSendDecideStep s.coordinator s.coordinator snd -> step s {s with coordinator := s.coordinator, network := {s.network with network := snd :: s.network.network}}
-| partRecvDec: ∀ s p2 i rcv, ParticipantReceiveDecisionStep (s.participants i) p2 rcv -> rcv ∈ s.network.network -> step s {s with participants := updateSet s.participants i p2, network := {s.network with network := s.network.network.erase rcv}}
+inductive step : System n -> System n -> Prop where
+| partSendPref: ∀ (s: System n) (i: Fin n) (p2: Participant n) (snd: Message n), ParticipantSendsPreference (s.participants i) p2 snd -> step s {s with participants := updateMap s.participants i p2, network := {s.network with network := snd :: s.network.network}}
+| coordRecvPref: ∀ (s: System n) (c2: Coordinator n) (rcv: Message n) , CoordinatorReceivesPreference s.coordinator c2 rcv -> rcv ∈ s.network.network-> step s {s with coordinator := c2, network := {s.network with network := s.network.network.erase rcv}}
+| coordMksDec: ∀ (s: System n) (c2: Coordinator n), CoordinatorMakesDecisionStep s.coordinator c2 -> step s {s with coordinator := c2}
+| coordSndDecStep: ∀ (s: System n) (snd: Message n), CoordinatorSendDecideStep s.coordinator s.coordinator snd -> step s {s with coordinator := s.coordinator, network := {s.network with network := snd :: s.network.network}}
+| partRecvDec: ∀ (s: System n) (p2: Participant n) (i: Fin n) (rcv: Message n), ParticipantReceiveDecisionStep (s.participants i) p2 rcv -> rcv ∈ s.network.network -> step s {s with participants := updateMap s.participants i p2, network := {s.network with network := s.network.network.erase rcv}}
 
-inductive steps : System -> System -> Prop where
+inductive steps : System n -> System n -> Prop where
 | refl : ∀ s1, steps s1 s1
 | trans: ∀ s1 s2 s3, steps s1 s2 -> step s2 s3 -> steps s1 s3 
 
-def validSystem (s: System) :=
+def validSystem (s: System n) :=
 ∃ s0, systemInits s0  ∧ steps s0 s
 
 
+theorem validSystemMapIds (s: System n) :
+validSystem s
+-> ∀ i, (s.participants i).hostid = i := by
+   intros sIsValid; unfold validSystem at sIsValid; rcases sIsValid with ⟨ s0, s0Inits, sSteps ⟩
+   induction sSteps
+   unfold systemInits participantInits at s0Inits; grind
+   rename_i s1 s2 sSteps sStep IH
+   cases sStep <;> try grind
+   rename_i i p m stepRule;simp [ParticipantSendsPreference] at stepRule; simp [updateMap]; grind
+   rename_i p i  m stepRule mInN ;simp [ParticipantReceiveDecisionStep] at stepRule; simp [updateMap]; grind
 
 
-theorem commitImpliesMessageSent (s0 s: System) :
+theorem commitImpliesMessageSent (s0 s: System n) :
     validSystem s0
     -> step s0 s 
     -> (∃ i, (s.participants i).decision = Decision.Commit)
@@ -71,17 +81,19 @@ theorem commitImpliesMessageSent (s0 s: System) :
     intros s0Valid sSteps sCommits
     cases sSteps with
     | partSendPref i p m stepRule =>
-      simp [ParticipantSendsPreference] at stepRule; simp at sCommits; rcases sCommits with ⟨ i', oldCommit⟩; unfold updateSet at oldCommit 
+      simp [ParticipantSendsPreference] at stepRule; simp at sCommits; rcases sCommits with ⟨ i', oldCommit⟩; unfold updateMap at oldCommit 
       grind
-    | partRecvDec  p i m stepRule net =>
-      simp [ParticipantReceiveDecisionStep] at stepRule; simp at sCommits;rcases sCommits with ⟨ i', oldCommit⟩; unfold updateSet at oldCommit; exists i'
+    | partRecvDec p i m stepRule net =>
+      simp [ParticipantReceiveDecisionStep] at stepRule; simp at sCommits;rcases sCommits with ⟨ i', oldCommit⟩; unfold updateMap at oldCommit; exists i'
       split at oldCommit <;> try grind
     | coordSndDecStep m stepRule =>
       grind
     | coordMksDec c stepRule => grind
     | coordRecvPref => grind
 
-theorem messageSentImplies (s: System) :
+
+
+theorem messageSentImplies (s: System n) :
     validSystem s ->
     Message.Decide Decision.Commit ∈ s.network.network
     -> s.coordinator.decision = Decision.Commit := by
@@ -91,14 +103,16 @@ theorem messageSentImplies (s: System) :
          unfold systemInits networkInits at s0Inits
          grind
        | trans s1 s2 s1Steps s2Step IH =>
-         cases s2Step <;> simp [CoordinatorSendDecideStep, CoordinatorSendDecideStep, CoordinatorMakesDecisionStep, CoordinatorReceivesPreference, ParticipantSendsPreference] at * <;> grind
+         cases s2Step <;> simp [CoordinatorSendDecideStep, CoordinatorSendDecideStep, CoordinatorMakesDecisionStep, CoordinatorReceivesPreference, ParticipantSendsPreference] at * <;> try grind
          
+       
+              
          
-theorem decisionImpliesVotes (s: System) :
+theorem decisionImpliesVotes (s: System n) :
     validSystem s 
     -> s.coordinator.decision = Decision.Commit
-    -> s.coordinator.yesVotes.count true == s.n := by
-       intro sValid messInNetwwork; unfold validSystem at sValid; rcases sValid  with ⟨ s0, s0Inits, sSteps ⟩
+    -> count s.coordinator.yesVotes == n := by
+       intro sValid messInNetwork; unfold validSystem at sValid; rcases sValid  with ⟨ s0, s0Inits, sSteps ⟩
        induction sSteps with
        | refl =>
          unfold systemInits coordinatorInits at s0Inits
@@ -113,17 +127,72 @@ theorem decisionImpliesVotes (s: System) :
          | coordMksDec c stepRule => simp [CoordinatorMakesDecisionStep] at stepRule; grind
          | coordRecvPref c m stepRule=>
            simp [CoordinatorReceivesPreference ] at *; rcases stepRule with ⟨pref, id, mNat, func⟩
-           sorry
+           split at func <;> try grind
+           subst_vars; simp at *
+           apply fullSetCannotIncrease; apply IH; apply messInNetwork
+           
 
-
-                       
+theorem yesVotesImpMessage (s_ s: System n) (i: Fin n):
+    validSystem s_
+    -> step s_ s
+    -> ∀ i, s.coordinator.yesVotes i = true 
+    -> s_.coordinator.yesVotes i = true ∨ Message.Vote Preference.Yes i ∈ s_.network.network := by
+       intros s0Valid stepS
+       cases stepS with
+       | partSendPref i p m stepRule =>
+           simp [ParticipantSendsPreference] at stepRule; grind
+       | partRecvDec  p i m stepRule net =>
+           simp [ParticipantReceiveDecisionStep] at stepRule; grind
+       | coordSndDecStep m stepRule => grind
+       | coordRecvPref c m stepRule =>
+         simp [CoordinatorReceivesPreference] at stepRule; simp; intro x
+         intros yesVotesIsTrue; rcases stepRule with ⟨p, i', mIsVote, funcFlow ⟩; split at funcFlow; subst_vars; simp [insertElem, updateMap] at yesVotesIsTrue <;> try grind
+         subst_vars; grind
+       | coordMksDec c stepRule =>
+         simp [CoordinatorMakesDecisionStep] at stepRule; rcases stepRule with ⟨ cIsNone, splitFun ⟩; split at splitFun
+         intros i cTrue; subst_vars; grind
+         intros i cTrue; subst_vars; simp at *; split at splitFun <;> try grind
+         subst_vars; simp at *; left; apply cTrue
          
          
+theorem messageSentImp (s: System n) (i: Fin n) :
+    validSystem s
+    -> Message.Vote Preference.Yes i ∈ s.network.network
+    -> (s.participants i).preference = Preference.Yes := by
+       intro sIsValid pInN; simp [validSystem] at sIsValid; rcases sIsValid with ⟨s0, s0Inits, sSteps⟩
+       induction sSteps
+       simp [systemInits, networkInits] at s0Inits; grind
+       rename_i s1 s2 steps1 step1 IH
+       cases step1 <;> simp [CoordinatorSendDecideStep, CoordinatorSendDecideStep, CoordinatorMakesDecisionStep, CoordinatorReceivesPreference, ParticipantSendsPreference, ParticipantReceiveDecisionStep] at * <;> try grind
+       rename_i i' p m sysInfo; rcases sysInfo with ⟨ eq1, eq2 ⟩; subst eq1 eq2; simp [updateMap]; split <;> try cases pInN <;> try grind
+       rename_i neq messEq; simp at messEq;
+       rw [validSystemMapIds] at messEq; grind; simp [validSystem]; grind
+       rename_i p n1  m rule messInN; rcases rule with ⟨ d, mDec ,decNone , pNat ⟩; subst_vars; simp [updateMap]; split <;> try grind
+       
+                   
+           
+theorem acceptImpliesMessageSent (s: System n) (i: Fin n):
+    validSystem s
+    -> s.coordinator.yesVotes i = true 
+    -> (s.participants i).preference = Preference.Yes := by
+       intro sIsvalid sCoord
+       sorry
+       
+       
 
-
-
+           
+theorem votesImpliesMessagesSent (s: System n):
+    validSystem s
+    -> n ≠ 0
+    -> count s.coordinator.yesVotes == n
+    -> ∀ i, (s.participants i).preference = Preference.Yes := by
+       intros validS neqZero coordTrue i
+       apply acceptImpliesMessageSent
+       grind; simp at *; apply fullSetImpN; grind;
+       
+       
 -- Final property we want to prove
-theorem commitImpliesPreference (s: System) :
+theorem commitImpliesPreference (s: System n) :
     validSystem s
     -> (∃ i, (s.participants i).decision = Decision.Commit)
     -> ∀ i, (s.participants i).preference = Preference.Yes := by
@@ -132,4 +201,4 @@ theorem commitImpliesPreference (s: System) :
     
     sorry
     
-    
+   
